src/opt/ProgressStep.v
@@ -30,7 +30,8 @@ Lemma progress_program_step
       (WF1: Local.wf lc1 mem1)
       (MEM1: Memory.closed mem1)
       (SC1: Memory.closed_timemap sc1 mem1)
-      (PROMISES1: lc1.(Local.promises) = Memory.bot):
+      (PROMISES1: lc1.(Local.promises) = Memory.bot)
+      (NOHALF1: Memory.no_half lc1.(Local.promises) mem1):
   exists e th2, <<STEP: Thread.program_step e (Thread.mk lang (State.mk rs1 (i1::s1)) lc1 sc1 mem1) th2>>.
 Proof.
   destruct i1.
@@ -44,12 +45,16 @@ Proof.
       { i. rewrite PROMISES1. apply Memory.bot_nonsynch_loc. }
       i. des. esplits. econs; [|econs 3]; eauto. econs. econs.
     + hexploit progress_read_step; eauto. i. des.
+      exploit Memory.no_half_bot_max_ts; eauto; i.
+      { rewrite <- PROMISES1. auto. }
       exploit Local.read_step_future; eauto. i. des.
       destruct (RegFile.eval_rmw rs1 rmw val) as [? []] eqn: EQ.
       * hexploit progress_write_step; eauto.
         { apply Time.incr_spec. }
-        { i. inv H. s. rewrite PROMISES1. apply Memory.bot_nonsynch_loc. }
-        i. des. esplits. econs; [|econs 4]; eauto. econs. econs. rewrite EQ. eauto.
+        { i. inv READ. s. rewrite PROMISES1. apply Memory.bot_nonsynch_loc. }
+        i. des. esplits. econs; [|econs 4]; eauto.
+        { econs. econs. rewrite EQ. eauto. }
+        { rewrite x0. eauto. }
       * esplits. econs; [|econs 2]; eauto. econs. econs. rewrite EQ; eauto.
     + hexploit progress_fence_step; eauto.
       { i. rewrite PROMISES1. apply Memory.bot_nonsynch. }
